<?xml version="1.0" encoding="UTF-8"?>

<rdf:RDF 
    xmlns:rdf="http://www.w3.org/1999/02/22-rdf-syntax-ns#"
    xmlns:rdfs="http://www.w3.org/2000/01/rdf-schema#" 
    xmlns:owl="http://www.w3.org/2002/07/owl#"
    xml:base="http://ld4l.org/ontology/core#">

    <!-- LD4L properties -->
    
    <owl:ObjectProperty rdf:about="http://ld4l.org/ontology/core#hasVcard">
        <rdfs:label>contact information</rdfs:label>
        <rdfs:comment>Relates a thing to its vCard (contact information).</rdfs:comment>
        <rdfs:range rdf:resource="http://www.w3.org/2006/vcard/ns#VCard" />
    </owl:ObjectProperty>
    
    <owl:ObjectProperty rdf:about="http://ld4l.org/ontology/core#vcardFor">
        <rdfs:label>contact information for</rdfs:label>
        <rdfs:comment>Relates a vCard (contact information) to the thing it belongs to.</rdfs:comment>
        <rdfs:domain rdf:resource="http://www.w3.org/2006/vcard/ns#VCard" />
        <owl:inverseOf rdfs:resource="http://ld4l.org/ontology/core#hasVcard" />        
    </owl:ObjectProperty>
    
    <!-- 
        For dealing with multiple identities associated with a single person 
        (e.g., pseudonyms. Currently using the vcard ontology instead. 
    -->
    <!--
    <owl:Class rdf:about="http://ld4l.org/ontology/core#Identity">
        <rdfs:label>Identity</rdfs:label>
        <rdfs:comment>An identity associated with a person (e.g., a pseudonym)</rdfs:comment>
        <rdfs:subClassOf rdf:resource="http://www.w3.org/2002/07/owl#Thing"/> (could have a more specific superclass)
    </owl:Class>
    
    <owl:ObjectProperty rdf:about="http://ld4l.org/ontology/core#hasAlternateIdentity">
        <rdfs:label>alternate name</rdfs:label>
        <rdfs:comment>Relates a thing to its pseudonym or other alternative identity.</rdfs:comment>
        <rdfs:range rdf:resource="http://www.w3.org/2006/vcard/ns#VCard" />
    </owl:ObjectProperty>
    
    <owl:ObjectProperty rdf:about="http://ld4l.org/ontology/core#alternateIdentityFor">
        <rdfs:label>alternate name for</rdfs:label>
        <rdfs:comment>Relates a pseudonym or other alternate identity to the thing it refers to.</rdfs:comment>
        <rdfs:domain rdf:resource="http://www.w3.org/2006/vcard/ns#VCard" />
        <owl:inverseOf rdfs:resource="http://ld4l.org/ontology/core#hasAlternateIdentity" />        
    </owl:ObjectProperty>
    -->
    
</rdf:RDF>